WIP

security/BtInfoAsm.v
@@ -56,9 +56,10 @@ Section BUNDLE.
   Variant bundle_event : Type :=
     (* generate a call code + other followup events; call-ext-ret *)
     | Bundle_call (tr: trace) (id: ident) (args: list eventval) (sg: signature)
-                  (d: option mem_delta)
+                  (d: mem_delta)
     (* generate a return code; ret *)
     | Bundle_return (tr: trace) (retv: eventval)
+                    (d: mem_delta)
     (* generate a builtin code; ext *)
     | Bundle_builtin (tr: trace) (ef: external_function) (args: list eventval)
                      (d: mem_delta)
@@ -68,7 +69,7 @@ Section BUNDLE.
 
   Definition unbundle (be: bundle_event): trace :=
     match be with
-    | Bundle_call tr _ _ _ _ | Bundle_return tr _ | Bundle_builtin tr _ _ _ => tr
+    | Bundle_call tr _ _ _ _ | Bundle_return tr _ _ | Bundle_builtin tr _ _ _ => tr
     end.
 
   Fixpoint unbundle_trace (btr: bundle_trace) : trace :=
@@ -200,7 +201,6 @@ Section IR.
 
   Definition ir_state := option (block * mem * ir_conts)%type.
 
-  (* TODO *)
   Variant ir_step (ge: Asm.genv) : ir_state -> bundle_event -> ir_state -> Prop :=
     | ir_step_cross_call_internal
         cur m1 ik
@@ -214,10 +214,12 @@ Section IR.
         (ALLOW: Genv.allowed_call ge cp (Vptr b Ptrofs.zero))
         (NPTR: crossing_comp ge cp cp' -> Forall not_ptr vargs)
         (SIG: sg = Asm.fn_sig f_next)
-        (* (PUB: public_first_order ge m1) *)
         (TR: call_trace_cross ge cp cp' b vargs (sig_args sg) tr id evargs)
+        d m2
+        (DELTA: mem_delta_apply_wf ge cp d (Some m1) = Some m2)
+        (PUB: public_first_order ge m2)
       :
-      ir_step ge (Some (cur, m1, ik)) (Bundle_call tr id evargs sg None) (Some (b, m1, (ir_cont cur) :: ik))
+      ir_step ge (Some (cur, m1, ik)) (Bundle_call tr id evargs sg d) (Some (b, m2, (ir_cont cur) :: ik))
     | ir_step_cross_return_internal
         cur m1 next ik ik_tl
         tr evretv
@@ -234,8 +236,11 @@ Section IR.
         (* internal return: memory changes in Clight-side, so need inj-relation *)
         (TR: return_trace_cross ge cp_next cp_cur vretv (sig_res sg) tr evretv)
         (CONT: ik = (ir_cont next) :: ik_tl)
+        d m2
+        (DELTA: mem_delta_apply_wf ge cp_cur d (Some m1) = Some m2)
+        (PUB: public_first_order ge m2)
       :
-      ir_step ge (Some (cur, m1, ik)) (Bundle_return tr evretv) (Some (next, m1, ik_tl))
+      ir_step ge (Some (cur, m1, ik)) (Bundle_return tr evretv d) (Some (next, m2, ik_tl))
     | ir_step_intra_call_external
         cur m1 m2 ik
         tr id evargs sg
@@ -248,21 +253,21 @@ Section IR.
         (INTRA: Genv.type_of_call ge cp_cur cp_ext = Genv.InternalCall)
         (SIG: sg = ef_sig ef)
         d m1'
-        (MEM: mem_delta_apply_inj (meminj_public ge) d (Some m1) = Some m1')
+        (MEM: mem_delta_apply_wf ge cp_cur d (Some m1) = Some m1')
         vargs vretv
         (EC: external_call ef ge vargs m1' tr vretv m2)
         (ECCASES: (external_call_unknowns ef ge m1' vargs) \/
                     (external_call_known_observables ef ge m1' vargs tr vretv m2 /\ d = []))
         (ARGS: evargs = vals_to_eventvals ge vargs)
       :
-      ir_step ge (Some (cur, m1, ik)) (Bundle_call tr id evargs sg (Some d)) (Some (cur, m2, ik))
+      ir_step ge (Some (cur, m1, ik)) (Bundle_call tr id evargs sg d) (Some (cur, m2, ik))
     | ir_step_builtin
         cur m1 m2 ik
         tr ef evargs
         cp_cur
         (CURCP: cp_cur = Genv.find_comp ge (Vptr cur Ptrofs.zero))
         d m1'
-        (MEM: mem_delta_apply_inj (meminj_public ge) d (Some m1) = Some m1')
+        (MEM: mem_delta_apply_wf ge cp_cur d (Some m1) = Some m1')
         vargs vretv
         (EC: external_call ef ge vargs m1' tr vretv m2)
         (ECCASES: (external_call_unknowns ef ge m1' vargs) \/
@@ -285,7 +290,7 @@ Section IR.
         (SIG: sg = ef_sig ef)
         (TR: call_trace_cross ge cp cp' b vargs (sig_args sg) tr id evargs)
       :
-      ir_step ge (Some (cur, m1, ik)) (Bundle_call tr id evargs sg None) None
+      ir_step ge (Some (cur, m1, ik)) (Bundle_call tr id evargs sg []) None
     | ir_step_cross_call_external2
         (* early cut at call-ext_call *)
         cur m1 ik
@@ -302,14 +307,14 @@ Section IR.
         (TR1: call_trace_cross ge cp cp' b vargs (sig_args sg) tr1 id evargs)
         (* external function part *)
         d m1'
-        (MEM: mem_delta_apply_inj (meminj_public ge) d (Some m1) = Some m1')
+        (MEM: mem_delta_apply_wf ge cp d (Some m1) = Some m1')
         tr2 m2 vretv
         (TR2: external_call ef ge vargs m1' tr2 vretv m2)
         (ECCASES: (external_call_unknowns ef ge m1' vargs) \/
                     (external_call_known_observables ef ge m1' vargs tr2 vretv m2 /\ d = []))
         (ARGS: evargs = vals_to_eventvals ge vargs)
       :
-      ir_step ge (Some (cur, m1, ik)) (Bundle_call (tr1 ++ tr2) id evargs sg (Some d)) None
+      ir_step ge (Some (cur, m1, ik)) (Bundle_call (tr1 ++ tr2) id evargs sg d) None
     | ir_step_cross_call_external3
         (* early cut at call-ext_call *)
         cur m1 ik
@@ -326,7 +331,7 @@ Section IR.
         (TR1: call_trace_cross ge cp cp' b vargs (sig_args sg) tr1 id evargs)
         (* external function part *)
         d m1'
-        (MEM: mem_delta_apply_inj (meminj_public ge) d (Some m1) = Some m1')
+        (MEM: mem_delta_apply_wf ge cp d (Some m1) = Some m1')
         tr2 m2 vretv
         (TR2: external_call ef ge vargs m1' tr2 vretv m2)
         (ECCASES: (external_call_unknowns ef ge m1' vargs) \/
@@ -339,7 +344,7 @@ Section IR.
         (INTERNAL: Genv.find_funct_ptr ge cur = Some (AST.Internal f_cur))
         (TR3: return_trace_cross ge cp cp' vretv (sig_res sg) tr3 evretv)
       :
-      ir_step ge (Some (cur, m1, ik)) (Bundle_call (tr1 ++ tr2 ++ tr3) id evargs sg (Some d)) (Some (cur, m2, ik)).
+      ir_step ge (Some (cur, m1, ik)) (Bundle_call (tr1 ++ tr2 ++ tr3) id evargs sg d) (Some (cur, m2, ik)).
 
 End IR.
 
@@ -494,50 +499,6 @@ Section FROMASM.
     eapply Mem.free_range_perm in FREE. unfold Mem.range_perm in FREE.
     eapply NFREE. erewrite INJPUB. congruence. eapply Mem.perm_cur_max; apply FREE.
     instantiate (1:=lo). lia.
-  Qed.
-
-  Lemma mem_delta_exec_instr
-        (ge: genv) f i rs m cp rs' m'
-        (NFREE: public_not_freeable ge m)
-        (EXEC: exec_instr ge f i rs m cp = Next rs' m')
-        m0 d
-        (DELTA0: mem_delta_inj_wf (meminj_public ge) d)
-        (DELTA1: mem_delta_apply d (Some m0) = Some m)
-    :
-    exists d', (mem_delta_inj_wf (meminj_public ge) d') /\ (mem_delta_apply d' (Some m0) = Some m').
-  Proof.
-    destruct i; simpl in EXEC.
-    all: try (inv EXEC; eauto).
-    all: simpl_before_exists; eauto.
-    all: try
-           (match goal with
-            | H: context [Mem.alloc] |- _ => idtac
-            | H: context [Mem.free] |- _ => idtac
-            | H: Mem.store ?ch ?m ?b ?ofs ?v ?cp = _ |-  _ =>
-                exists (d ++ [mem_delta_kind_store (ch, b, ofs, v, cp)]); split
-            end;
-            [apply Forall_app; split; [auto | constructor; simpl; auto]
-            | rewrite mem_delta_apply_app; (match goal with | H: mem_delta_apply _ _ = Some _ |- _ => rewrite H end; simpl; auto) ]).
-    { match goal with
-      | _: Mem.alloc _ ?cp1 ?lo ?hi = _, _: Mem.store ?ch _ ?b ?ofs ?v ?cp2 = _ |- _ =>
-          exists (d ++ ([mem_delta_kind_alloc (cp1, lo, hi)] ++ [mem_delta_kind_store (ch, b, ofs, v, cp2)]))
-      end.
-      split.
-      - apply Forall_app; split; auto. apply Forall_app; split; constructor; simpl; auto.
-      - rewrite mem_delta_apply_app. rewrite DELTA1. rewrite mem_delta_apply_app. simpl. rewrite Heqp. simpl. auto.
-    }
-    { destruct (Z.leb_spec sz 0); cycle 1.
-      { match goal with
-        | _: Mem.free _ ?b ?lo ?hi ?cp = _ |- _ =>
-            exists (d ++ [mem_delta_kind_free (b, lo, hi, cp)])
-        end.
-        split.
-        - apply Forall_app; split; auto. constructor; auto. simpl. destruct (meminj_public ge b) eqn:INJPUB; auto. exfalso.
-          eapply Mem.free_range_perm in Heqo0. unfold Mem.range_perm in Heqo0. eapply NFREE. erewrite INJPUB. congruence. eapply Mem.perm_cur_max; apply Heqo0. instantiate (1:=0%Z). lia.
-        - rewrite mem_delta_apply_app. rewrite DELTA1. simpl. auto.
-      }
-      { apply Mem.free_result in Heqo0. unfold Mem.unchecked_free in Heqo0. unfold zle in Heqo0. des_ifs. eexists; eauto. }
-    }
   Qed.
 
   Lemma public_not_freeable_store
@@ -701,6 +662,8 @@ Section FROMASM.
     revert m0 NALLOC m1 APPD. induction d; intros.
     { simpl in *. inv APPD. auto. }
     rewrite mem_delta_apply_cons in APPD. destruct a.
+    - destruct d0 as (((ch & ptr) & v) & cp). ss. exploit mem_delta_apply_some. eapply APPD. intros (mi & MEM). rewrite MEM in APPD. eapply IHd. 2: eapply APPD.
+      unfold meminj_not_alloc in *. intros. eapply NALLOC. destruct ptr; ss. erewrite Mem.nextblock_store in H; eauto.
     - destruct d0 as ((((ch & b) & ofs) & v) & cp). simpl in *. exploit mem_delta_apply_some. eapply APPD. intros (mi & MEM). rewrite MEM in APPD. eapply IHd. 2: eapply APPD.
       unfold meminj_not_alloc in *. intros. eapply NALLOC. erewrite Mem.nextblock_store in H; eauto.
     - destruct d0 as (((b & ofs) & mvs) & cp). simpl in *. exploit mem_delta_apply_some. eapply APPD. intros (mi & MEM). rewrite MEM in APPD. eapply IHd. 2: eapply APPD.
@@ -727,6 +690,53 @@ Section FROMASM.
     :
     (rs' X1 = Val.offset_ptr rs#PC Ptrofs.one) /\ (m' = m).
   Proof. destruct i; simpl in *; clarify. Qed.
+
+  Lemma mem_delta_exec_instr
+        (ge: genv) f i rs m cp rs' m'
+        (NFREE: public_not_freeable ge m)
+        (EXEC: exec_instr ge f i rs m cp = Next rs' m')
+        m0 d
+        (DELTA0: mem_delta_inj_wf cp (meminj_public ge) d)
+        (DELTA1: mem_delta_apply d (Some m0) = Some m)
+        (NALLOC: meminj_not_alloc (meminj_public ge) m0)
+    :
+    exists d', (mem_delta_inj_wf cp (meminj_public ge) d') /\ (mem_delta_apply d' (Some m0) = Some m').
+  Proof.
+    destruct i; simpl in EXEC.
+    all: try (inv EXEC; eauto).
+    all: simpl_before_exists; eauto.
+    all: try
+           (match goal with
+            | H: context [Mem.alloc] |- _ => idtac
+            | H: context [Mem.free] |- _ => idtac
+            | H: Mem.store ?ch ?m ?b (Ptrofs.unsigned ?ofs) ?v ?cp = _ |-  _ =>
+                exists (d ++ [mem_delta_kind_storev (ch, Vptr b ofs, v, cp)]); split
+            end;
+            [apply Forall_app; split; [auto | constructor; ss; auto]
+            | rewrite mem_delta_apply_app; (match goal with | H: mem_delta_apply _ _ = Some _ |- _ => rewrite H end; simpl; auto) ]).
+    { match goal with
+      | _: Mem.alloc _ ?cp1 ?lo ?hi = _, _: Mem.store ?ch _ ?b ?ofs ?v ?cp2 = _ |- _ =>
+          exists (d ++ ([mem_delta_kind_alloc (cp1, lo, hi)] ++ [mem_delta_kind_store (ch, b, ofs, v, cp2)]))
+      end.
+      split.
+      - apply Forall_app; split; auto. apply Forall_app; split; constructor; simpl; auto.
+        hexploit meminj_not_alloc_delta. eauto. eapply DELTA1. intros NALLOC2. apply NALLOC2.
+        exploit Mem.alloc_result; eauto. lia.
+      - rewrite mem_delta_apply_app. rewrite DELTA1. rewrite mem_delta_apply_app. simpl. rewrite Heqp. simpl. auto.
+    }
+    { destruct (Z.leb_spec sz 0); cycle 1.
+      { match goal with
+        | _: Mem.free _ ?b ?lo ?hi ?cp = _ |- _ =>
+            exists (d ++ [mem_delta_kind_free (b, lo, hi, cp)])
+        end.
+        split.
+        - apply Forall_app; split; auto. constructor; auto. simpl. destruct (meminj_public ge b) eqn:INJPUB; auto. exfalso.
+          eapply Mem.free_range_perm in Heqo0. unfold Mem.range_perm in Heqo0. eapply NFREE. erewrite INJPUB. congruence. eapply Mem.perm_cur_max; apply Heqo0. instantiate (1:=0%Z). lia.
+        - rewrite mem_delta_apply_app. rewrite DELTA1. simpl. auto.
+      }
+      { apply Mem.free_result in Heqo0. unfold Mem.unchecked_free in Heqo0. unfold zle in Heqo0. des_ifs. eexists; eauto. }
+    }
+  Qed.
 
 End FROMASM.
 
@@ -798,11 +808,11 @@ Section INVS.
     :
     match_stack ge (ir_cont next :: ik_tl) (Stackframe b cp sg v ofs :: sk_tl).
 
-  Definition match_mem (ge: Senv.t) (k: meminj) (d: mem_delta) (m_a0 m_i m_a1: mem): Prop :=
+  Definition match_mem (ge: Senv.t) cp (k: meminj) (d: mem_delta) (m_a0 m_i m_a1: mem): Prop :=
     let j := meminj_public ge in
     (Mem.inject k m_a0 m_i) /\ (inject_incr j k) /\
       (meminj_not_alloc j m_a0) /\ (public_not_freeable ge m_a1) /\
-      (mem_delta_inj_wf j d) /\ (mem_delta_apply d (Some m_a0) = Some m_a1) /\
+      (mem_delta_inj_wf cp j d) /\ (mem_delta_apply d (Some m_a0) = Some m_a1) /\
       (public_rev_perm ge m_a1 m_i).
 
   Definition match_state (ge: Asm.genv) (k: meminj) (m_a0: mem) (d: mem_delta) (ast: Asm.state) (ist: ir_state): Prop :=
@@ -810,7 +820,7 @@ Section INVS.
     | State sk rs m_a, Some (cur, m_i, ik) =>
         (wf_ir_cur ge cur) /\ (wf_ir_conts ge ik) /\
           (match_cur_stack_sig cur ge sk) /\ (match_cur_regset cur ge rs) /\
-          (match_stack ge ik sk) /\ (match_mem ge k d m_a0 m_i m_a)
+          (match_stack ge ik sk) /\ (match_mem ge (Genv.find_comp ge (Vptr cur Ptrofs.zero)) k d m_a0 m_i m_a)
     | _, _ => False
     end.
 
@@ -908,19 +918,20 @@ Section PROOF.
   Qed.
 
   Lemma public_rev_perm_delta_apply_inj
-        d ge m m_i m_i'
+        d ge m m_i m_i' cp
         (PRP: public_rev_perm ge m m_i)
-        (APPD: mem_delta_apply_inj (meminj_public ge) d (Some m_i) = Some m_i')
+        (APPD: mem_delta_apply_wf ge cp d (Some m_i) = Some m_i')
     :
     public_rev_perm ge m m_i'.
   Proof.
     revert_until d. induction d; intros.
-    { ss; clarify. }
-    rewrite mem_delta_apply_inj_cons in APPD. des_ifs; clarify; eauto.
-    exploit mem_delta_apply_inj_some; eauto. intros (m1 & STORE). rewrite STORE in APPD.
+    { unfold mem_delta_apply_wf in APPD. ss. clarify. }
+    rewrite mem_delta_apply_wf_cons in APPD. des_ifs; clarify; eauto.
+    exploit mem_delta_apply_wf_some; eauto. intros (m1 & STORE). rewrite STORE in APPD.
     eapply IHd; clear IHd. 2: eauto.
-    unfold public_rev_perm in *. intros. specialize (PRP b1). des_ifs. intros.
-    eapply PRP. ss. eapply Mem.perm_store_2; eauto.
+    unfold public_rev_perm in *. intros. specialize (PRP b). des_ifs. intros.
+    eapply PRP. unfold wf_mem_delta_kind_b in Heq. des_ifs. ss. unfold mem_delta_apply_storev in STORE. des_ifs.
+    destruct v0; ss. eapply Mem.perm_store_2; eauto.
   Qed.
 
   Lemma mem_perm_any_to_nonempty
@@ -975,23 +986,23 @@ Section PROOF.
   Qed.
 
   Lemma match_mem_external_call_establish1
-        (ge: genv) k d m_a0 m_i m
-        (MEM: match_mem ge k d m_a0 m_i m)
+        (ge: genv) cp k d m_a0 m_i m
+        (MEM: match_mem ge cp k d m_a0 m_i m)
         ef args t res m'
         (EXTCALL: external_call ef ge args m t res m')
         (ECC: external_call_unknowns ef ge m args)
     :
     exists m1 m2 res',
-      (mem_delta_apply_inj (meminj_public ge) d (Some m_i) = Some m1) /\
+      (mem_delta_apply_wf ge cp d (Some m_i) = Some m1) /\
         (external_call ef ge args m1 t res' m2) /\
         (external_call_unknowns ef ge m1 args) /\
-        (exists k2, match_mem ge k2 [] m' m2 m' /\ Val.inject k2 res res')
+        (exists k2, match_mem ge cp k2 [] m' m2 m' /\ Val.inject k2 res res')
   .
   Proof.
     destruct MEM as (MEM0 & MEM1 & MEM2 & MEM3 & MEM4 & MEM5 & MEM6).
     (* reestablish meminj *)
     exploit mem_delta_apply_establish_inject; eauto.
-    { apply meminj_public_strict. }
+    (* { apply meminj_public_strict. } *)
     { eapply external_call_unknowns_fo. eauto. }
     intros (m_i' & APPD' & MEMINJ').
     hexploit ec_mem_inject. eapply external_call_spec. 2: eapply EXTCALL. all: eauto.
@@ -999,7 +1010,7 @@ Section PROOF.
     { instantiate (1:=ge). apply symbols_inject_meminj_public. }
     { instantiate (1:=args). eapply external_call_unknowns_val_inject_list; eauto. }
     intros (f' & vres' & m_i'' & EXTCALL' & VALINJ' & MEMINJ'' & _ & _ & INCRINJ' & _).
-    assert (MM': match_mem ge f' [] m' m_i'' m').
+    assert (MM': match_mem ge cp f' [] m' m_i'' m').
     { unfold match_mem. simpl.
       assert (PNF: public_not_freeable ge m').
       { pose proof (meminj_not_alloc_delta _ _ MEM2 _ _ MEM5) as NALLOC.
@@ -1065,7 +1076,7 @@ Section PROOF.
         (CURCOMP : Genv.find_comp ge (Vptr cur Ptrofs.zero) = callee_comp cpm st)
         (MTST2 : match_stack ge ik st)
         k d m_a0 m_i m_a
-        (MEM: match_mem ge k d m_a0 m_i m_a)
+        (MEM: match_mem ge (Genv.find_comp ge (Vptr cur Ptrofs.zero)) k d m_a0 m_i m_a)
         t' ast'
         (STEP: step_fix cpm ge (ReturnState st rs m_a) t' ast')
         t'' ast''
@@ -1108,15 +1119,15 @@ Section PROOF.
   Qed.
 
   Lemma match_mem_external_call_establish2
-        ge k d m_a0 m_i m
-        (MEM: match_mem ge k d m_a0 m_i m)
+        ge cp k d m_a0 m_i m
+        (MEM: match_mem ge cp k d m_a0 m_i m)
         ef args t res m'
         (EXTCALL: external_call ef ge args m t res m')
         (ECKO: external_call_known_observables ef ge m args t res m')
     :
     (external_call ef ge args m_i t res m_i) /\
       (external_call_known_observables ef ge m_i args t res m_i) /\
-      (match_mem ge k d m_a0 m_i m')
+      (match_mem ge cp k d m_a0 m_i m')
   .
   Proof.
     destruct MEM as (MEM0 & MEM1 & MEM2 & MEM3 & MEM4 & MEM5 & MEM6).
@@ -1141,17 +1152,17 @@ Section PROOF.
   Qed.
 
   Lemma match_mem_external_call_establish
-        (ge: genv) k d m_a0 m_i m
-        (MEM: match_mem ge k d m_a0 m_i m)
+        (ge: genv) cp k d m_a0 m_i m
+        (MEM: match_mem ge cp k d m_a0 m_i m)
         ef args t res m'
         (EXTCALL: external_call ef ge args m t res m')
         (ECC: external_call_unknowns ef ge m args \/ external_call_known_observables ef ge m args t res m')
     :
     exists d' m1 m2 res',
-      (mem_delta_apply_inj (meminj_public ge) d' (Some m_i) = Some m1) /\
+      (mem_delta_apply_wf ge cp d' (Some m_i) = Some m1) /\
         (external_call ef ge args m1 t res' m2) /\
         ((external_call_unknowns ef ge m1 args) \/ (external_call_known_observables ef ge m1 args t res' m2 /\ d' = [])) /\
-        (exists k2 d2 m_a02, match_mem ge k2 d2 m_a02 m2 m' /\ (Val.inject k2 res res' \/ (res = res')))
+        (exists k2 d2 m_a02, match_mem ge cp k2 d2 m_a02 m2 m' /\ (Val.inject k2 res res' \/ (res = res')))
   .
   Proof.
     destruct ECC as [ECC | ECC].
@@ -1171,7 +1182,7 @@ Section PROOF.
         (CURCOMP : Genv.find_comp ge (Vptr cur Ptrofs.zero) = callee_comp cpm st)
         (MTST2 : match_stack ge ik st)
         k d m_a0 m_i m_a
-        (MEM: match_mem ge k d m_a0 m_i m_a)
+        (MEM: match_mem ge (Genv.find_comp ge (Vptr cur Ptrofs.zero)) k d m_a0 m_i m_a)
         t ast'
         (STEP: step_fix cpm ge (State st rs m_a) t ast')
         b1 ofs1
@@ -1184,7 +1195,7 @@ Section PROOF.
     exists (btr : bundle_trace) k' d' m_a0' m_i' m_a',
       (unbundle_trace btr = t) /\
         (istar ir_step ge (Some (cur, m_i, ik)) btr (Some (cur, m_i', ik))) /\
-        (match_mem ge k' d' m_a0' m_i' m_a') /\
+        (match_mem ge (Genv.find_comp ge (Vptr cur Ptrofs.zero)) k' d' m_a0' m_i' m_a') /\
         (exists res, star_measure (step_fix cpm) ge n
                              (ReturnState st (set_pair (loc_external_result (ef_sig ef)) res (undef_caller_save_regs rs)) # PC <- (rs X1) m_a') t' ast'').
   Proof.
@@ -1202,7 +1213,7 @@ Section PROOF.
     - (* extcall is unknown *)
       exploit match_mem_external_call_establish1; eauto. unfold match_mem; splits; eauto.
       intros. des.
-      exists ([Bundle_call t ef_id (vals_to_eventvals ge args) (ef_sig ef0) (Some d)]).
+      exists ([Bundle_call t ef_id (vals_to_eventvals ge args) (ef_sig ef0) (d)]).
       do 5 eexists. splits; simpl. 3: eapply x3. apply app_nil_r.
       2:{ exists res. auto. }
       econstructor 2. 2: econstructor 1. 2: eauto.
@@ -1215,24 +1226,24 @@ Section PROOF.
       rename H4 into EXTCALL, H7 into EXTARGS. unfold external_call_known_observables in ECKO.
       des_ifs; simpl in *.
       { destruct ECKO as [_ OBS]. inv EXTCALL. inv H; simpl in *; clarify.
-        exists ([Bundle_call [Event_vload chunk id ofs ev] ef_id [EVptr_global id ofs] {| sig_args := [Tptr]; sig_res := rettype_of_chunk chunk; sig_cc := cc_default |} (Some [])]).
+        exists ([Bundle_call [Event_vload chunk id ofs ev] ef_id [EVptr_global id ofs] {| sig_args := [Tptr]; sig_res := rettype_of_chunk chunk; sig_cc := cc_default |} ([])]).
         exists k, d, m_a0, m_i, m'. simpl. splits; auto. 2: split; auto. 2: eauto.
         econstructor 2. 2: econstructor 1. 2: auto.
         eapply ir_step_intra_call_external. all: eauto.
         { rewrite CURCOMP, <- REC_CURCOMP, NEXTPC. simpl. unfold Genv.find_comp. setoid_rewrite NEXTF. unfold Genv.type_of_call. rewrite Pos.eqb_refl. auto. }
-        { simpl. eauto. }
+        { ss. }
         { simpl. econstructor. econstructor 1; eauto. }
         { simpl. right. split; auto. econs; eauto. econs. econs; eauto. }
         { simpl. unfold senv_invert_symbol_total. erewrite Senv.find_invert_symbol; eauto. }
         splits; auto.
       }
       { destruct ECKO as [_ OBS]. inv EXTCALL. inv H; simpl in *; clarify.
-        exists ([Bundle_call [Event_vstore chunk id ofs ev] ef_id [EVptr_global id ofs; ev] {| sig_args := [Tptr; type_of_chunk chunk]; sig_res := Tvoid; sig_cc := cc_default |} (Some [])]).
+        exists ([Bundle_call [Event_vstore chunk id ofs ev] ef_id [EVptr_global id ofs; ev] {| sig_args := [Tptr; type_of_chunk chunk]; sig_res := Tvoid; sig_cc := cc_default |} ([])]).
         exists k, d, m_a0, m_i, m'. simpl. splits; auto. 2: split; auto. 2: eauto.
         econstructor 2. 2: econstructor 1. 2: auto.
         eapply ir_step_intra_call_external. all: eauto.
         { rewrite CURCOMP, <- REC_CURCOMP, NEXTPC. simpl. unfold Genv.find_comp. setoid_rewrite NEXTF. unfold Genv.type_of_call. rewrite Pos.eqb_refl. auto. }
-        { simpl. eauto. }
+        { ss. }
         { instantiate (2:=[Vptr b0 ofs; Val.load_result chunk v]).
           simpl. econstructor. econstructor 1; eauto. rewrite val_load_result_idem. auto.
         }
@@ -1246,23 +1257,23 @@ Section PROOF.
       { destruct ECKO as [_ OBS]. inv EXTCALL; clarify. }
       { destruct ECKO as [_ OBS]. inv EXTCALL; clarify. }
       { destruct ECKO as [_ OBS]. inv EXTCALL; simpl in *; clarify.
-        exists ([Bundle_call [Event_annot text args0] ef_id (vals_to_eventvals ge args) {| sig_args := targs; sig_res := Tvoid; sig_cc := cc_default |} (Some [])]).
+        exists ([Bundle_call [Event_annot text args0] ef_id (vals_to_eventvals ge args) {| sig_args := targs; sig_res := Tvoid; sig_cc := cc_default |} ([])]).
         exists k, d, m_a0, m_i, m'. simpl. splits; auto. 2: split; auto. 2: eauto.
         econstructor 2. 2: econstructor 1. 2: auto.
         eapply ir_step_intra_call_external. all: eauto.
         { rewrite CURCOMP, <- REC_CURCOMP, NEXTPC. simpl. unfold Genv.find_comp. setoid_rewrite NEXTF. unfold Genv.type_of_call. rewrite Pos.eqb_refl. auto. }
-        { simpl. eauto. }
+        { ss. }
         { simpl. econstructor. auto. }
         { simpl. right. split; auto. econs; eauto. econs. auto. }
         splits; auto.
       }
       { destruct ECKO as [_ OBS]. inv EXTCALL; simpl in *; clarify.
-        exists ([Bundle_call [Event_annot text [arg]] ef_id [val_to_eventval ge res] {| sig_args := [targ]; sig_res := targ; sig_cc := cc_default |} (Some [])]).
+        exists ([Bundle_call [Event_annot text [arg]] ef_id [val_to_eventval ge res] {| sig_args := [targ]; sig_res := targ; sig_cc := cc_default |} ([])]).
         exists k, d, m_a0, m_i, m'. simpl. splits; auto. 2: split; auto. 2: eauto.
         econstructor 2. 2: econstructor 1. 2: auto.
         eapply ir_step_intra_call_external. all: eauto.
         { rewrite CURCOMP, <- REC_CURCOMP, NEXTPC. simpl. unfold Genv.find_comp. setoid_rewrite NEXTF. unfold Genv.type_of_call. rewrite Pos.eqb_refl. auto. }
-        { simpl. eauto. }
+        { ss. }
         { simpl. econstructor. eauto. }
         { simpl. right. split; auto. econs; eauto. econs. auto. }
         { simpl. auto. }
@@ -1283,9 +1294,11 @@ Section PROOF.
         exists [], k, d, m_a0, m_i, m'. simpl. splits; auto. 2: unfold match_mem; splits; auto. 2: eauto. econstructor 1.
       }
       { destruct ECKS as [_ OBS]. inv EXTCALL. inv H; simpl in *; clarify.
-        exists [], k, (d ++ [mem_delta_kind_store (chunk, b0, (Ptrofs.unsigned ofs), v, cp)]), m_a0, m_i, m'. simpl. splits; auto. econstructor 1. 2: eauto. unfold match_mem. splits; auto.
+        exists [], k, (d ++ [mem_delta_kind_storev (chunk, Vptr b0 ofs, v, cp)]), m_a0, m_i, m'. simpl. splits; auto. econstructor 1. 2: eauto. unfold match_mem. splits; auto.
         { eapply public_not_freeable_store; eauto. }
-        { setoid_rewrite Forall_app. split; auto. econs; auto. simpl. auto. }
+        { setoid_rewrite Forall_app. split; auto. econs; auto. ss.
+          rewrite CURCOMP. rewrite <- REC_CURCOMP. rewrite NEXTPC. ss. unfold Genv.find_comp. setoid_rewrite NEXTF. ss.
+        }
         { rewrite mem_delta_apply_app. rewrite MEM5. simpl. auto. }
         { eapply public_rev_perm_store; eauto. }
       }
@@ -1298,7 +1311,8 @@ Section PROOF.
         }
         { setoid_rewrite Forall_app. split; auto. econs; auto.
           { simpl. auto. }
-          econs; auto. simpl. auto.
+          econs; auto. simpl. hexploit Mem.alloc_result; eauto. hexploit meminj_not_alloc_delta; eauto.
+          intros. apply H1. lia.
         }
         { rewrite mem_delta_apply_app. rewrite MEM5. simpl. rewrite H. simpl. auto. }
         { eapply public_rev_perm_store. 2: eauto. eapply public_rev_perm_alloc.
@@ -1356,7 +1370,7 @@ Section PROOF.
     exists (btr : bundle_trace) k' d' m_a0' m_i',
       (unbundle_trace btr = t1) /\
         (istar ir_step ge (Some (cur, m_i, ik)) btr (Some (cur, m_i', ik))) /\
-        (match_mem ge k' d' m_a0' m_i' m').
+        (match_mem ge (Genv.find_comp ge (Vptr cur Ptrofs.zero)) k' d' m_a0' m_i' m').
   Proof.
     ss. destruct MTST as (WFIR0 & WFIR1 & MTST0 & MTST1 & MTST2 & MTST3).
     destruct MTST3 as (MEM0 & MEM1 & MEM2 & MEM3 & MEM4 & MEM5 & MEM6).
@@ -1379,7 +1393,7 @@ Section PROOF.
         exists k, d, m_a0, m_i. simpl. splits; auto. 2: split; auto.
         econstructor 2. 2: econstructor 1. 2: auto.
         eapply ir_step_builtin. all: eauto.
-        { simpl. eauto. }
+        { ss. }
         { simpl. econstructor. econstructor 1; eauto. }
         { simpl. right. split; auto. econs; eauto. econs. econs; eauto. }
         { simpl. unfold senv_invert_symbol_total. erewrite Senv.find_invert_symbol; eauto. }
@@ -1390,7 +1404,7 @@ Section PROOF.
         exists k, d, m_a0, m_i. simpl. splits; auto. 2: split; auto.
         econstructor 2. 2: econstructor 1. 2: auto.
         eapply ir_step_builtin. all: eauto.
-        { simpl. eauto. }
+        { ss. }
         { instantiate (2:=[Vptr b0 ofs0; Val.load_result chunk v]).
           simpl. econstructor. econstructor 1; eauto. rewrite val_load_result_idem. auto.
         }
@@ -1408,7 +1422,7 @@ Section PROOF.
         exists k, d, m_a0, m_i. simpl. splits; auto. 2: split; auto.
         econstructor 2. 2: econstructor 1. 2: auto.
         eapply ir_step_builtin. all: eauto.
-        { simpl. eauto. }
+        { ss. }
         { simpl. econstructor. auto. }
         { simpl. right. split; auto. econs; eauto. econs. auto. }
         splits; auto.
@@ -1418,7 +1432,7 @@ Section PROOF.
         exists k, d, m_a0, m_i. simpl. splits; auto. 2: split; auto.
         econstructor 2. 2: econstructor 1. 2: auto.
         eapply ir_step_builtin. all: eauto.
-        { simpl. eauto. }
+        { ss. }
         { simpl. econstructor. eauto. }
         { simpl. right. split; auto. econs; eauto. econs. auto. }
         { simpl. auto. }
@@ -1438,9 +1452,11 @@ Section PROOF.
         exists [], k, d, m_a0, m_i. simpl. splits; auto. 2: rr; splits; auto. econstructor 1.
       }
       { destruct ECKS as [_ OBS]. inv EXTCALL. inv H; simpl in *; clarify.
-        exists [], k, (d ++ [mem_delta_kind_store (chunk, b0, (Ptrofs.unsigned ofs0), v, cp)]), m_a0, m_i. simpl. splits; auto. econstructor 1. unfold match_mem. splits; auto.
+        exists [], k, (d ++ [mem_delta_kind_storev (chunk, Vptr b0 ofs0, v, cp)]), m_a0, m_i. simpl. splits; auto. econstructor 1. unfold match_mem. splits; auto.
         { eapply public_not_freeable_store; eauto. }
-        { setoid_rewrite Forall_app. split; auto. econs; auto. simpl. auto. }
+        { setoid_rewrite Forall_app. split; auto. econs; auto. ss.
+          rewrite MTST1. rewrite CURPC. ss. unfold Genv.find_comp. setoid_rewrite CURF. auto.
+        }
         { rewrite mem_delta_apply_app. rewrite MEM5. simpl. auto. }
         { eapply public_rev_perm_store; eauto. }
       }
@@ -1453,7 +1469,8 @@ Section PROOF.
         }
         { setoid_rewrite Forall_app. split; auto. econs; auto.
           { simpl. auto. }
-          econs; auto. simpl. auto.
+          econs; auto. simpl. hexploit Mem.alloc_result; eauto. hexploit meminj_not_alloc_delta; eauto.
+          intros. apply H1. lia.
         }
         { rewrite mem_delta_apply_app. rewrite MEM5. simpl. rewrite H. simpl. auto. }
         { eapply public_rev_perm_store. 2: eauto. eapply public_rev_perm_alloc.
@@ -1516,7 +1533,7 @@ Section PROOF.
         (CURCOMP : Genv.find_comp ge (Vptr cur Ptrofs.zero) = callee_comp cpm st)
         (MTST2 : match_stack ge ik st)
         k d m_a0 m_i m_a
-        (MEM: match_mem ge k d m_a0 m_i m_a)
+        (MEM: match_mem ge (Genv.find_comp ge (Vptr cur Ptrofs.zero)) k d m_a0 m_i m_a)
         (RSX: rs X1 = Vundef)
         t' ast'
         (STEP: step_fix cpm ge (ReturnState st rs m_a) t' ast')
@@ -1600,7 +1617,7 @@ Section PROOF.
         (CURCOMP : Genv.find_comp ge (Vptr cur Ptrofs.zero) = callee_comp cpm st)
         (MTST2 : match_stack ge ik st)
         k d m_a0 m_i m_a
-        (MEM: match_mem ge k d m_a0 m_i m_a)
+        (MEM: match_mem ge (Genv.find_comp ge (Vptr cur Ptrofs.zero)) k d m_a0 m_i m_a)
         t' ast'
         (STEP: step_fix cpm ge (ReturnState st rs m_a) t' ast')
         t'' ast''
@@ -1613,32 +1630,56 @@ Section PROOF.
     (** step --- ReturnState *)
     inv STEP. inv EV; simpl in *.
     { rewrite CCC in H. congruence with H. }
-    clear H.
+    clear H. specialize (CHECKPUB CCC).
     (** return is ccc --- next is poped from the stack, which is internal, so done *)
     unfold Genv.type_of_call in CCC. des_ifs. clear CCC. unfold update_stack_return in STUPD.
     rewrite Pos.eqb_sym in Heq. rewrite Heq in STUPD. des_ifs.
     pose proof Heq as NEQ. eapply Pos.eqb_neq in NEQ. specialize (PC_RA NEQ).
     destruct s as [b3 cp3 sig3 rv3 ptr3]. simpl in *.
     inv WFASM1. simpl in *. des_ifs. clear H2. inv MTST2.
+    hexploit mem_delta_apply_establish_inject. eapply MEM0. 1,2,3,4: eauto.
+    { clear - CHECKPUB. ii. unfold public_first_order in CHECKPUB. unfold meminj_public in H. des_ifs.
+      eapply CHECKPUB; eauto. apply Senv.invert_find_symbol; auto.
+    }
+    intros (m_i' & APPD & MEMINJ).
     exploit (IH _ _ _ _ _ _ _ _ STAR). lia. all: auto.
     { simpl. split; auto. unfold wf_regset. rewrite PC_RA. rewrite Heq0. auto. }
-    { instantiate (4:=k). instantiate (3:=m_a0). instantiate (2:=d).
-      instantiate (1:=Some (next, m_i, ik_tl)). simpl. splits; auto.
+    { instantiate (4:=(meminj_public ge)). instantiate (3:=m_a). instantiate (2:=[]).
+      instantiate (1:=Some (next, m_i', ik_tl)). simpl. splits; auto.
       { inv WFIR1. simpl in *. auto. }
       { inv WFIR1. auto. }
       { unfold match_cur_regset. rewrite COMP. rewrite PC_RA. auto. }
-      { rr; splits; auto. }
+      { rr; splits; auto. eapply meminj_not_alloc_delta; eauto. ss. eapply public_rev_perm_delta_apply_inj; eauto.
+      }
     }
+    (* { instantiate (4:=k). instantiate (3:=m_a0). instantiate (2:=d). *)
+    (*   instantiate (1:=Some (next, m_i, ik_tl)). simpl. splits; auto. *)
+    (*   { inv WFIR1. simpl in *. auto. } *)
+    (*   { inv WFIR1. auto. } *)
+    (*   { unfold match_cur_regset. rewrite COMP. rewrite PC_RA. auto. } *)
+    (*   { rr; splits; auto. } *)
+    (* } *)
     intros (btr & ist' & UTR & ISTAR').
-    exists ((Bundle_return [Event_return (Genv.find_comp_ignore_offset ge (rs PC)) (Genv.find_comp ge (Vptr cur Ptrofs.zero)) res] res) :: btr), ist'.
+    exists ((Bundle_return [Event_return (Genv.find_comp_ignore_offset ge (rs PC)) (Genv.find_comp ge (Vptr cur Ptrofs.zero)) res] res d) :: btr), ist'.
+    (* exists ((Bundle_return [Event_return (Genv.find_comp_ignore_offset ge (rs PC)) (Genv.find_comp ge (Vptr cur Ptrofs.zero)) res] res) :: btr), ist'. *)
     simpl. rewrite UTR. split; auto.
     econstructor 2. 2: eapply ISTAR'. 2: auto.
     inv WFIR1. simpl in *. des_ifs. clear H2. unfold wf_ir_cur in WFIR0. des_ifs. clear WFIR0.
     eapply ir_step_cross_return_internal. 6: eapply Heq1. all: eauto.
     { rewrite COMP. rewrite PC_RA. simpl. auto. }
-    constructor; auto.
-    { unfold Genv.type_of_call. rewrite Pos.eqb_sym, Heq. auto. }
-    { replace (funsig (Internal f2)) with sig3; auto. unfold match_cur_stack_sig in MTST0. des_ifs. }
+    { constructor; auto.
+      { unfold Genv.type_of_call. rewrite Pos.eqb_sym, Heq. auto. }
+      { replace (funsig (Internal f2)) with sig3; auto. unfold match_cur_stack_sig in MTST0. des_ifs. }
+    }
+    { hexploit public_rev_perm_delta_apply_inj. eauto. eapply APPD. intros REVP. clear - MEMINJ CHECKPUB REVP.
+      unfold public_first_order in *. i.
+      exploit Senv.find_invert_symbol; eauto. intros INV.
+      assert (PERM: Mem.perm m_a b ofs Cur Readable).
+      { specialize (REVP b). unfold meminj_public in REVP. rewrite INV, PUBLIC in REVP. apply REVP. rewrite Z.add_0_r. auto. }
+      eapply loc_first_order_memval_inject_preserves. eapply CHECKPUB; eauto.
+      instantiate (1:=ge). inv MEMINJ. inv mi_inj. replace ofs with (ofs + 0)%Z at 2 by lia. eapply mi_memval; auto.
+      unfold meminj_public. rewrite INV, PUBLIC. auto.
+    }
   Qed.
 
   Lemma asm_to_ir_returnstate_undef
@@ -1663,7 +1704,7 @@ Section PROOF.
         (CURCOMP : Genv.find_comp ge (Vptr cur Ptrofs.zero) = callee_comp cpm st)
         (MTST2 : match_stack ge ik st)
         k d m_a0 m_i m_a
-        (MEM: match_mem ge k d m_a0 m_i m_a)
+        (MEM: match_mem ge (Genv.find_comp ge (Vptr cur Ptrofs.zero)) k d m_a0 m_i m_a)
         (RSX: rs X1 = Vundef)
         t' ast'
         (STEP: step_fix cpm ge (ReturnState st rs m_a) t' ast')
@@ -1720,7 +1761,7 @@ Section PROOF.
         (CURCOMP : Genv.find_comp ge (Vptr cur Ptrofs.zero) = callee_comp cpm st)
         (MTST2 : match_stack ge ik st)
         k d m_a0 m_i m_a
-        (MEM: match_mem ge k d m_a0 m_i m_a)
+        (MEM: match_mem ge (Genv.find_comp ge (Vptr cur Ptrofs.zero)) k d m_a0 m_i m_a)
         t' ast'
         (STEP: step_fix cpm ge (ReturnState st rs m_a) t' ast')
         t'' ast''
@@ -1787,7 +1828,7 @@ Section PROOF.
         (CURCOMP : Genv.find_comp ge (Vptr cur Ptrofs.zero) = callee_comp cpm st)
         (MTST2 : match_stack ge ik st)
         k d m_a0 m_i m_a
-        (MEM: match_mem ge k d m_a0 m_i m_a)
+        (MEM: match_mem ge (Genv.find_comp ge (Vptr cur Ptrofs.zero)) k d m_a0 m_i m_a)
         t' ast'
         (STEP: step_fix cpm ge (ReturnState st rs m_a) t' ast')
         t'' ast''
@@ -1830,8 +1871,9 @@ Section PROOF.
               wf_ge ge ->
               wf_asm ge ast ->
               star_measure (step_fix cpm) ge y ast tr ast' ->
-              forall (ist : ir_state) (k : meminj) (d : mem_delta), match_state ge k m_a0 d ast ist ->
-                                                               exists (btr : bundle_trace) (ist' : ir_state), unbundle_trace btr = tr /\ istar ir_step ge ist btr ist')
+              forall (ist : ir_state) (k : meminj) (d : mem_delta),
+                match_state ge k m_a0 d ast ist ->
+                exists (btr : bundle_trace) (ist' : ir_state), unbundle_trace btr = tr /\ istar ir_step ge ist btr ist')
         m_a0 ast'
         (WFGE: wf_ge ge)
         rs m st
@@ -1840,12 +1882,7 @@ Section PROOF.
         (MTST: match_state ge k m_a0 d (State st rs m) ist)
         t2 rs' m'
         (STAR: star_measure (step_fix cpm) ge n (State st rs' m') t2 ast')
-        b
-        ofs
-        f
-        i
-        b'
-        ofs'
+        b ofs f i b' ofs'
         (H0: rs PC = Vptr b ofs)
         (H1: Genv.find_funct_ptr ge b = Some (Internal f))
         (H2: find_instr (Ptrofs.unsigned ofs) (fn_code f) = Some i)
@@ -1869,7 +1906,11 @@ Section PROOF.
     unfold match_state in MTST. destruct ist as [[[cur m_i] ik] |].
     2:{ inv MTST. }
     destruct MTST as (WFIR0 & WFIR1 & MTST0 & MTST1 & MTST2 & MTST3). destruct MTST3 as (MEM0 & MEM1 & MEM2 & MEM3 & MEM4 & MEM5 & MEM6).
-    exploit mem_delta_exec_instr. eapply MEM3. eapply H3. eapply MEM4. eapply MEM5. intros (d' & MEM4' & MEM5').
+    exploit mem_delta_exec_instr. eapply MEM3. eapply H3.
+    { replace (comp_of f) with (Genv.find_comp ge (Vptr cur Ptrofs.zero)). eapply MEM4.
+      rewrite MTST1. rewrite H0. ss. unfold Genv.find_comp. setoid_rewrite H1. auto.
+    }
+    eapply MEM5. auto. intros (d' & MEM4' & MEM5').
     destruct f0.
 
     (** has next function --- internal *)
@@ -1886,6 +1927,9 @@ Section PROOF.
         split. auto.
         { unfold match_mem. splits; auto.
           eapply public_not_freeable_exec_instr. 3: eapply H3. all: auto. eapply meminj_not_alloc_delta; eauto.
+          { replace (Genv.find_comp ge (Vptr cur Ptrofs.zero)) with (comp_of f); auto.
+            rewrite MTST1. rewrite H0. ss. unfold Genv.find_comp. setoid_rewrite H1. auto.
+          }
           eapply public_rev_perm_exec_instr. 3: eapply H3. all: auto.
         }
       }
@@ -1906,6 +1950,9 @@ Section PROOF.
       }
       { instantiate (4:=k). instantiate (3:=d'). unfold match_mem. splits; eauto.
         eapply public_not_freeable_exec_instr; eauto. eapply meminj_not_alloc_delta; eauto.
+        { replace (Genv.find_comp ge (Vptr cur Ptrofs.zero)) with (comp_of f); auto.
+          rewrite MTST1. rewrite H0. ss. unfold Genv.find_comp. setoid_rewrite H1. auto.
+        }
         eapply public_rev_perm_exec_instr; eauto.
       }
       intros (btr' & k' & d'0 & m_a0' & m_i' & m_a' & UTR' & ISTAR' & MM' & (res' & STAR')).
@@ -2037,7 +2084,7 @@ Section PROOF.
       { destruct ist as [[[cur m_i] ik] |]; ss.
         destruct MTST as (WFIR0 & WFIR1 & MTST0 & MTST1 & MTST2 & MTST3).
         destruct WFASM as [WFASM0 WFASM1].
-        assert (Genv.CrossCompartmentCall <> Genv.InternalCall) by congruence. specialize (CALLSIG H); clear H. des.
+        specialize (CALLSIG eq_refl). des.
         exploit exec_instr_is_call; eauto. clear H2 H3 H4. intros (RSX & MEM). subst m'.
         destruct fd.
         (* calling internal function *)
@@ -2049,12 +2096,29 @@ Section PROOF.
           2:{ instantiate (2:=[Event_call (comp_of f) (Genv.find_comp ge (Vptr b0 Ptrofs.zero)) i0 vl]). simpl. eauto. }
           assert (EQC2: (Genv.find_comp ge (Vptr b0 Ptrofs.zero)) = comp_of f0).
           { unfold Genv.find_comp. setoid_rewrite CALLSIG. auto. }
-          exists ([Bundle_call [Event_call (comp_of f) (Genv.find_comp ge (Vptr b0 Ptrofs.zero)) i0 vl] i0 vl (fn_sig f0) None]). eexists. split.
+          specialize (CHECKPUB eq_refl).
+          pose proof MTST3 as MEM. destruct MEM as (MEM0 & MEM1 & MEM2 & MEM3 & MEM4 & MEM5 & MEM6).
+          hexploit mem_delta_apply_establish_inject. eapply MEM0. 1,2,3,4: eauto.
+          { clear - CHECKPUB. ii. unfold public_first_order in CHECKPUB. unfold meminj_public in H. des_ifs.
+            eapply CHECKPUB; eauto. apply Senv.invert_find_symbol; auto.
+          }
+          intros (m_i' & APPD & MEMINJ).
+          exists ([Bundle_call [Event_call (comp_of f) (Genv.find_comp ge (Vptr b0 Ptrofs.zero)) i0 vl] i0 vl (fn_sig f0) d]). eexists. split.
           { simpl. split; auto. econstructor 2. 2: econstructor 1. 2: eauto. eapply ir_step_cross_call_internal.
             7: eauto. 6: intros; eapply NO_CROSS_PTR; auto. 3: setoid_rewrite CALLSIG; auto. 3,4: eauto.
             { rewrite MTST1. rewrite <- EQC, H0. simpl. auto. }
             { apply Genv.invert_find_symbol; auto. }
             { econs; auto. }
+            { replace (comp_of f) with (Genv.find_comp ge (Vptr cur Ptrofs.zero)). eapply APPD. rewrite MTST1. rewrite H0. ss. }
+            { hexploit public_rev_perm_delta_apply_inj. eauto. eapply APPD. intros REVP. clear - MEMINJ CHECKPUB REVP.
+              unfold public_first_order in *. i.
+              exploit Senv.find_invert_symbol; eauto. intros INV.
+              assert (PERM: Mem.perm m b ofs Cur Readable).
+              { specialize (REVP b). unfold meminj_public in REVP. rewrite INV, PUBLIC in REVP. apply REVP. rewrite Z.add_0_r. auto. }
+              eapply loc_first_order_memval_inject_preserves. eapply CHECKPUB; eauto.
+              instantiate (1:=ge). inv MEMINJ. inv mi_inj. replace ofs with (ofs + 0)%Z at 2 by lia. eapply mi_memval; auto.
+              unfold meminj_public. rewrite INV, PUBLIC. auto.
+            }
           }
           rewrite H0 in RSX. simpl in RSX. inv RSX.
           eapply IH. 4: eapply STAR. all: auto.
@@ -2068,6 +2132,8 @@ Section PROOF.
           - unfold match_cur_stack_sig. rewrite CALLSIG. ss.
           - unfold match_cur_regset. rewrite NEXTPC. ss.
           - econs; eauto. rewrite MTST1. rewrite H0. ss.
+          - instantiate (3:=(meminj_public ge)). instantiate (2:=[]). instantiate (1:=m).
+            rr; splits; auto. eapply meminj_not_alloc_delta; eauto. ss. eapply public_rev_perm_delta_apply_inj; eauto.
         }
         (* calling external function *)
         { assert (EQC2: (Genv.find_comp ge (Vptr b' Ptrofs.zero)) = comp_of e).
